

Basic Differentiation :

$$y = ax^n$$

$\frac{dy}{dx} = anx^{n-1}$

e.g.:

$$\textcircled{1} y = 5x^2$$

$$\begin{aligned} \frac{dy}{dx} &= (5 \times 2) x^{2-1} \\ &= 10x^1 \\ &= 10x. \end{aligned}$$

Differentiate $\rightarrow x^1$,

$y = x$	$y = 2x$	$y = -3x$	$y = \frac{5}{3}x$
$\frac{dy}{dx} = 1$	$\frac{dy}{dx} = 2$	$\frac{dy}{dx} = -3$	$\frac{dy}{dx} = \frac{5}{3}$

Differentiate \rightarrow constant

$y = 1$	$y = -1$	$y = 1/3$
$\frac{dy}{dx} = 0$	$\frac{dy}{dx} = 0$	$\frac{dy}{dx} = 0$

Differentiate multiple:

$$\odot y = 2x^2 + 5x + 2 + 3x^3$$

$$\frac{dy}{dx} = 4x + 5 + 0 + 9x^2$$

$$\frac{dy}{dx} = 4x + 5 + 9x^2$$

Differentiate with chain rule:

method (i) :-

$$y = (2x^2 + 5x + 2)^{10}$$

let,

$$u = 2x^2 + 5x + 2 \quad \text{--- (i)}$$

$$y = u^{10} \quad \text{--- (ii)}$$

$$\therefore \frac{dy}{dx} = \frac{d}{dx} \text{ (i)} \times \frac{d}{du} \text{ (ii)}$$

$$= \frac{d}{dx} (2x^2 + 5x + 2) \times \frac{d}{du} (u)^{10}$$

$$= (4x + 5) \times 10u^9$$

Replace u with actual value \rightarrow

$$= (4x+5) \times 10 (2x^2+5x+2)^9$$

$$= 10 (4x+5) (2x^2+5x+2)^9$$

Differentiation with different alphabets: \rightarrow

$$y = 2x^2 + 5x$$

$$y = 2u^2 + 5u$$

u, y, x
are all
variables

$$\frac{dy}{dx} = 4x + 5$$

$$\frac{dy}{du} = 4u + 5$$

$$x = 2y^2 + 5y$$

$$u = 2x^2 + 5x + 2$$

$$\frac{dx}{dy} = 4y + 5$$

$$\frac{du}{dx} = 4x + 5$$

Differentiation, where a, b and c are constant:

$$y = 2ax^2 + bx + c$$

$$t = 2ax^2 + bx + c,$$

here, b is not a constant.
as it is not mentioned.
It is a variable here.

$$\frac{dy}{dx} = 4ax + b$$

$$(2a \times 2)x^{2-1}$$

$$\therefore \frac{dt}{dx} = 4ax + b$$

method (ii): Chain rule.

$$y = (2x^2 + 5x + 2)^{10}$$

Let, $u = 2x^2 + 5x + 2$.

Formula: $y = u^{10}$

$$\frac{dy}{dx} = \frac{dy}{du} \times \frac{du}{dx}$$

for $\frac{dy}{du}$, we need to find an equation

such as $y = u^5 + 2u^2 \dots$

We have in our question,

$y = u^{10}$

$$\frac{dy}{du} = 10u^9$$

for $\frac{du}{dx}$, $u = 2x^2 + 5x \dots$

We have, $u = 2x^2 + 5x + 2$

$$\frac{du}{dx} = 4x + 5$$

$$\therefore y = (2x^2 + 5x + 2)^{10}$$

$$\frac{dy}{dx} = \frac{dy}{du} \times \frac{du}{dx}$$

$$= 10u^9 \times (4x + 5)$$

Replace u , with $u = 2x^2 + 5x + 2$

$$\frac{dy}{dx} = 10(2x^2 + 5x + 2)^9 (4x + 5).$$

Answer.